start POSTP

theories/StackMachines/BSM/TM_computable_to_BSM_computable.v
@@ -25,17 +25,37 @@ Proof.
   - intros t H % Hb3 % Hb2 % Hb1. exact H.
 Qed.
 
+Definition bsm_addstacks n (P : list (bsm_instr n)) m : list (bsm_instr (m + n)):=
+  map (fun x => match x with 
+  | bsm_pop x c1 c2 => bsm_pop (pos_right m x) c1 c2
+  | bsm_push x b => bsm_push (pos_right m x) b end) P.
+
+
+Lemma vec_pos_spec {k} {X} (p : pos k) (v : Vector.t X k) : vec_pos v p = Vector.nth v p.
+Proof.
+  induction v in p |- *.
+  - inversion p.
+  - eapply (Fin.caseS' p).
+    + reflexivity.
+    + intros. cbn. eauto.
+Qed.
+
 Lemma BSM_addstacks n i (P : list (bsm_instr n)) m : 
-   {P' | (forall j v o v', BSM.eval n (i, P) (j, v) (o, v') -> forall v'', BSM.eval (m + n) (i, P') (j, Vector.append v'' v) (o, Vector.append v'' v'))
+   {P' | length P = length P' /\ (forall j v o v', BSM.eval n (i, P) (j, v) (o, v') -> forall v'', BSM.eval (m + n) (i, P') (j, Vector.append v'' v) (o, Vector.append v'' v'))
           /\ forall v v'' j out, BSM.eval (m + n) (i, P') (j, Vector.append v'' v) out -> exists out, BSM.eval n (i, P) (j, v) out}.
 Proof.
-Admitted.  
-
-Lemma BSM_addstacks' n i (P : list (bsm_instr n)) m m' : 
-   {P' | length P = length P' /\
-   (forall j v o v', BSM.eval n (i, P) (j, v) (o, v') -> forall v'' v''', BSM.eval (m + (m' + n)) (i, P') (j, Vector.append v'' (Vector.append v''' v)) (o, Vector.append v'' (Vector.append v''' v')))
-          /\ forall v v'' v''' j out, BSM.eval (m + (m' + n)) (i, P') (j, Vector.append v'' (Vector.append v''' v)) out -> exists out, BSM.eval n (i, P) (j, v) out}.
-Proof.
+  exists (bsm_addstacks P m). split. { unfold bsm_addstacks. now rewrite map_length. } split.
+  - intros j v o v' H v''.  remember (i, P) as iP. remember (j, v) as jv. remember (o, v') as ov'.
+    replace i with (fst iP) by now rewrite HeqiP.
+    replace P with (snd iP) by now rewrite HeqiP.
+    replace j with (fst jv) by now rewrite Heqjv.
+    replace v with (snd jv) by now rewrite Heqjv.
+    replace o with (fst ov') by now rewrite Heqov'.
+    replace v' with (snd ov') by now rewrite Heqov'.
+    induction H in * |- *; cbn in *.
+    + econstructor 1. now rewrite map_length.
+    + econstructor 2. lia.
+      2:{ rewrite <- vec_app_spec. rewrite !vec_pos_app_right. 
 Admitted.  
 
 Definition encode_bsm (Σ : finType) n (t : Vector.t (tape Σ) n) :=
@@ -43,26 +63,10 @@ Definition encode_bsm (Σ : finType) n (t : Vector.t (tape Σ) n) :=
 Arguments encode_bsm {_ _} _, _ {_} _.
 
 Lemma encode_bsm_nil (Σ : finType) n   :
-  { '( str1, str2, n') | str1 = nil /\ forall (t : Vector.t (tape Σ) n),
-      encode_bsm Σ (niltape ::: t) = 
-     [| str1 ++ (encode_bsm Σ t)@[Fin0]; (encode_bsm Σ t)@[Fin1]; str2 ++ (skipn n' ((encode_bsm Σ t)@[Fin2])); (encode_bsm Σ t)@[Fin3] |]}.
+  { '(str2, n') | forall (t : Vector.t (tape Σ) n), (encode_bsm Σ (niltape ::: t))@[Fin2] =  str2 ++ (skipn n' ((encode_bsm Σ t)@[Fin2]))}.
 Proof.
-  eexists (_, _, _). split. shelve. cbn. intros t.
-  unfold encode_bsm at 1.
-  unfold enc_tape at 1. repeat f_equal.
-  - unfold complete_encode. unfold conv_tape.
-    etransitivity.
-    destruct destruct_vector_cons as (? & ? & E). inv E. cbn.
-    destruct_tapes. cbn. reflexivity.
-    symmetry. etransitivity.
-    destruct destruct_vector_cons as (? & ? & E). inv E. cbn.
-    destruct_tapes. cbn. reflexivity. instantiate (1 := []). reflexivity.
-  - unfold complete_encode, conv_tape.
-    etransitivity.
-    destruct destruct_vector_cons as (? & ? & E). inv E. cbn.
-    destruct_tapes. cbn. reflexivity.
-    destruct destruct_vector_cons as (? & ? & E). inv E. cbn. reflexivity.
-  - unfold complete_encode, conv_tape.
+  eexists (_, _). cbn. intros t.
+  unfold complete_encode, conv_tape.
     etransitivity.
     destruct destruct_vector_cons as (? & ? & E). inv E. cbn - [skipn].
     destruct_tapes. cbn - [skipn]. reflexivity.
@@ -73,7 +77,6 @@ Proof.
   
     instantiate (1 := encode_sym _ ++ true :: false :: encode_sym _ ++ true :: false :: encode_sym _). cbn.
     rewrite <- app_assoc. cbn. now rewrite <- app_assoc.
-    Unshelve. reflexivity.
 Qed.
 
 Definition strpush_common_short (Σ : finType) (s b : Σ) :=
@@ -201,35 +204,35 @@ Proof.
   rewrite <- app_assoc. cbn. rewrite <- app_assoc. cbn. rewrite <- app_assoc. cbn. rewrite <- app_assoc. cbn. rewrite <- app_assoc. cbn. reflexivity.
 Qed.
 
-Lemma BSM_complete_simulation' n Σ (M : TM Σ n) m m' i :
+Lemma BSM_complete_simulation' n Σ (M : TM Σ n) m i :
 { P |
       (forall q t t', TM.eval M (TM.start M) t q t' -> 
-       forall v'' v''', BSM.eval (m + (m' + 4)) (i, P) (i, Vector.append v'' (Vector.append v''' (encode_bsm t))) (i + length P, Vector.append v'' (Vector.append v''' (encode_bsm t')))) /\
-      (forall t v'' v''', (exists out, BSM.eval (m + (m' + 4)) (i, P) (i, Vector.append v'' (Vector.append v''' (encode_bsm t))) out) -> (exists q' t', TM.eval M (TM.start M) t q' t'))}.
+       forall v'', BSM.eval (m + (4)) (i, P) (i, Vector.append v'' ((encode_bsm t))) (i + length P, Vector.append v'' ((encode_bsm t')))) /\
+      (forall t v'', (exists out, BSM.eval (m + (4)) (i, P) (i, Vector.append v'' ((encode_bsm t))) out) -> (exists q' t', TM.eval M (TM.start M) t q' t'))}.
 Proof.
   destruct (SBTM_complete_simulation M) as (M1 & Hf1 & Hb1).
-  destruct (BSM_addstacks' i (SIM M1 i) m m') as (M2 & Hl & Hf2 & Hb2).
+  destruct (BSM_addstacks i (SIM M1 i) m ) as (M2 & Hl & Hf2 & Hb2).
   exists M2. split.
   - intros q t t' [q1 H % (SIM_computes i) ] % Hf1.
     intros. eapply Hf2. eapply BSM_sss.eval_iff. split.
     cbn [Fin.to_nat proj1_sig mult] in H. rewrite !NPeano.Nat.add_0_l, NPeano.Nat.add_0_r in H.
     rewrite <- Hl. rewrite SIM_length. rewrite mult_comm. eapply H.
     right. unfold fst, subcode.code_end, snd, fst. rewrite <- Hl. lia.
-  - intros t v'' v''' (out & [[out1 out2] [Ho1 Ho2]% BSM_sss.eval_iff] % Hb2). eapply Hb1.
+  - intros t v'' (out & [[out1 out2] [Ho1 Ho2]% BSM_sss.eval_iff] % Hb2). eapply Hb1.
     eapply SIM_term with (q := Fin.F1) in Ho2 .
     2:{ cbn [Fin.to_nat proj1_sig mult]. rewrite !NPeano.Nat.add_0_l, NPeano.Nat.add_0_r. eapply Ho1. }
     destruct Ho2 as (q' & t' & H1 & -> & H2). eauto.
 Qed.  
 
-Lemma BSM_complete_simulation n Σ (M : TM Σ n) m m' i :
+Lemma BSM_complete_simulation n Σ (M : TM Σ n) m  i :
 { P |
       (forall q t t', TM.eval M (TM.start M) t q t' -> 
-       forall v'' v''', BSM.eval (m + (m' + 4)) (i, P) (i, Vector.append v'' (Vector.append v''' (encode_bsm t))) (i + length P, Vector.append v'' (Vector.append v''' (encode_bsm t')))) /\
-      (forall t v'' v''', (sss.sss_terminates (bsm_sss (n := (m + (m' + 4)))) (i, P) (i, Vector.append v'' (Vector.append v''' (encode_bsm t)))) -> (exists q' t', TM.eval M (TM.start M) t q' t'))}.
+       forall v'', BSM.eval (m + (4)) (i, P) (i, Vector.append v'' ((encode_bsm t))) (i + length P, Vector.append v'' ((encode_bsm t')))) /\
+      (forall t v'', (sss.sss_terminates (bsm_sss (n := (m + (4)))) (i, P) (i, Vector.append v'' ((encode_bsm t)))) -> (exists q' t', TM.eval M (TM.start M) t q' t'))}.
 Proof.
-  destruct (@BSM_complete_simulation' n Σ M m m' i) as (P & H1 & H2).
+  destruct (@BSM_complete_simulation' n Σ M m i) as (P & H1 & H2).
   exists P. split. exact H1.
-  intros t v'' v''' ([out1 out2] & H % BSM_sss.eval_iff). eapply H2. eauto.
+  intros t v'' ([out1 out2] & H % BSM_sss.eval_iff). eapply H2. eauto.
 Qed. 
 
 Local Notation "P // s ->> t" := (sss_compute (@bsm_sss _) P s t).
@@ -276,14 +279,6 @@ Proof.
   induction p; cbn; eauto.
 Qed.
 
-Lemma vec_pos_spec {k} {X} (p : pos k) (v : Vector.t X k) : vec_pos v p = Vector.nth v p.
-Proof.
-  induction v in p |- *.
-  - inversion p.
-  - eapply (Fin.caseS' p).
-    + reflexivity.
-    + intros. cbn. eauto.
-Qed.
 
 Lemma Fin4_cases (P : pos 4 -> Prop) :
    P Fin0 -> P Fin1 -> P Fin2 -> P Fin3 -> forall p, P p.
@@ -293,20 +288,20 @@ Proof.
   intros p. inversion p.
 Qed.
 
-Lemma PREP1_spec k Σ  : 
+Lemma PREP1_spec k Σ n : 
 { PREP1 : list (bsm_instr ((1 + k) + 4)) | forall v : Vector.t nat k, 
     (0, PREP1) // (0, Vector.append ([] ::: Vector.map (fun n0 : nat => repeat true n0) v) (Vector.const [] 4)) ->>
-                  (length PREP1, Vector.append ([] ::: Vector.map (fun n0 : nat => repeat true n0) v) ((@encode_bsm Σ _ (Vector.const niltape 4)))) }.
+                  (length PREP1, Vector.append ([] ::: Vector.map (fun n0 : nat => repeat true n0) v) ((@encode_bsm Σ _ (Vector.const niltape n)))) }.
 Proof.
-  exists (push_exactly (pos_right (1 + k) Fin0) ((@encode_bsm Σ _ (Vector.const niltape 4))@[Fin0])
-       ++ push_exactly (pos_right (1 + k) Fin1) ((@encode_bsm Σ _ (Vector.const niltape 4))@[Fin1])
-       ++ push_exactly (pos_right (1 + k) Fin2) ((@encode_bsm Σ _ (Vector.const niltape 4))@[Fin2])
-       ++ push_exactly (pos_right (1 + k) Fin3) ((@encode_bsm Σ _ (Vector.const niltape 4))@[Fin3])).
+  exists (push_exactly (pos_right (1 + k) Fin0) ((@encode_bsm Σ _ (Vector.const niltape n))@[Fin0])
+       ++ push_exactly (pos_right (1 + k) Fin1) ((@encode_bsm Σ _ (Vector.const niltape n))@[Fin1])
+       ++ push_exactly (pos_right (1 + k) Fin2) ((@encode_bsm Σ _ (Vector.const niltape n))@[Fin2])
+       ++ push_exactly (pos_right (1 + k) Fin3) ((@encode_bsm Σ _ (Vector.const niltape n))@[Fin3])).
   intros v.
-  eapply subcode_sss_compute_trans. 2: eapply (push_exactly_spec (pos_right (1 + k) Fin0) 0 ((@encode_bsm Σ _ (Vector.const niltape 4))@[Fin0])). 1:auto.
-  eapply subcode_sss_compute_trans. 2: eapply (push_exactly_spec (pos_right (1 + k) Fin1) _ ((@encode_bsm Σ _ (Vector.const niltape 4))@[Fin1])). 1:auto.
-  eapply subcode_sss_compute_trans. 2: eapply (push_exactly_spec (pos_right (1 + k) Fin2) _ ((@encode_bsm Σ _ (Vector.const niltape 4))@[Fin2])). 1:auto.
-  eapply subcode_sss_compute_trans. 2: eapply (push_exactly_spec (pos_right (1 + k) Fin3) _ ((@encode_bsm Σ _ (Vector.const niltape 4))@[Fin3])). 1:auto.
+  eapply subcode_sss_compute_trans. 2: eapply (push_exactly_spec (pos_right (1 + k) Fin0) 0 ((@encode_bsm Σ _ (Vector.const niltape n))@[Fin0])). 1:auto.
+  eapply subcode_sss_compute_trans. 2: eapply (push_exactly_spec (pos_right (1 + k) Fin1) _ ((@encode_bsm Σ _ (Vector.const niltape n))@[Fin1])). 1:auto.
+  eapply subcode_sss_compute_trans. 2: eapply (push_exactly_spec (pos_right (1 + k) Fin2) _ ((@encode_bsm Σ _ (Vector.const niltape n))@[Fin2])). 1:auto.
+  eapply subcode_sss_compute_trans. 2: eapply (push_exactly_spec (pos_right (1 + k) Fin3) _ ((@encode_bsm Σ _ (Vector.const niltape n))@[Fin3])). 1:auto.
   bsm sss stop. f_equal.
   1:rewrite !app_length; lia.
   eapply vec_pos_ext. eapply pos_left_right_rect. 
@@ -490,17 +485,17 @@ Proof.
   destruct E. cbn. now rewrite !cast_eq_refl.
 Qed.
 
-Fixpoint PREP2' (Σ : finType) (s b : Σ) k'' (k' : nat)  (i : nat) : list (bsm_instr ((1 + (k' + k'') + 4))).
+Fixpoint PREP2' (Σ : finType) (s b : Σ) k'' (k' : nat)  (i : nat) (n : nat) : list (bsm_instr ((1 + (k' + k'') + 4))).
 Proof.
   destruct k'.
   - exact List.nil.
-  - refine (List.app _ (BSM_cast (PREP2' Σ s b (S k'') k' (i + PREP2''_length s b)) _)). 2:abstract lia.
+  - refine (List.app _ (BSM_cast (PREP2' Σ s b (S k'') k' (i + PREP2''_length s b) n) _)). 2:abstract lia.
     assert (k' < S k' + k'') as Hn by abstract lia.
-    refine (proj1_sig (@PREP2_spec' (S k' + k'') Σ (Fin.of_nat_lt Hn) i s b (k'' + 4))).
+    refine (proj1_sig (@PREP2_spec' (S k' + k'') Σ (Fin.of_nat_lt Hn) i s b (k'' + n))).
 Defined.
 
-Lemma PREP2'_length (Σ : finType) (s b : Σ) k (k' : nat) (i : nat) :
-  | @PREP2' Σ s b k k' i | = k' * PREP2''_length s b.
+Lemma PREP2'_length (Σ : finType) (s b : Σ) k (k' : nat) (i : nat) n :
+  | @PREP2' Σ s b k k' i n| = k' * PREP2''_length s b.
 Proof.
   induction k' in k, i |- *.
   - cbn. reflexivity.
@@ -513,12 +508,16 @@ Notation "v1 +++ v2" := (Vector.append v1 v2) (at level 60).
 Lemma vec_list_encode_bsm Σ n1 n2 v1 v2 :
 vec_list v1 = vec_list v2 ->
  vec_list (@encode_bsm Σ n1 v1) = vec_list (@encode_bsm Σ n2 v2).
-Admitted.
+Proof.
+  intros H.
+  assert (n1 = n2). eapply (f_equal (@length _)) in H. rewrite !vec_list_length in H. eauto. 
+  subst. eapply vec_list_inj in H. now subst.
+Qed.
 
-Lemma PREP2_spec_strong k (Σ : finType) (x : pos k) i s b k' k'' v (v' : Vector.t nat k'') (t : Vector.t (tape Σ) 4) : 
-    (i, @PREP2' Σ s b k'' k'  i) //
+Lemma PREP2_spec_strong (Σ : finType) i s b k' k'' v (v' : Vector.t nat k'') n (t : Vector.t (tape Σ) n) : 
+    (i, @PREP2' Σ s b k'' k'  i n) //
         (i,                                            ([] ::: Vector.map (fun n => repeat true n) v +++ Vector.const [] k'') +++  (@encode_bsm Σ _ (Vector.map (encNatTM s b) v' +++ t))) ->>
-        (i + length(@PREP2' Σ s b k'' k' i), ([] ::: Vector.const [] (k' + k'')  +++  (@encode_bsm Σ _ (Vector.map (encNatTM s b) (v +++ v') +++ t)))).
+        (i + length(@PREP2' Σ s b k'' k' i n), ([] ::: Vector.const [] (k' + k'')  +++  (@encode_bsm Σ _ (Vector.map (encNatTM s b) (v +++ v') +++ t)))).
 Proof.
   induction k' in k'', v, v', i |- *.
   - cbn. bsm sss stop. f_equal. lia. f_equal. revert v. eapply (Vector.case0). cbn. reflexivity.
@@ -526,8 +525,8 @@ Proof.
     assert (k' < S k') as Hlt by lia.
     match goal with [ |- context[proj1_sig ?y]] => destruct y as [PREPIT [HlP HPREP]]; cbn [proj1_sig] end.
     eapply subcode_sss_compute_trans with (P := (i, _)). { cbn - [minus mult]. eexists [], _. cbn - [mult minus]. split. reflexivity. cbn; now rewrite NPeano.Nat.add_0_r. }
-    cbn - [minus mult]. cbn - [minus mult] in HPREP.  replace (S (k' + k'') - S k' + 4) with (k'' + 4) in HPREP by lia. eapply HPREP with (m := v@[Fin.of_nat_lt Hlt]).
-    Arguments Fin.of_nat_lt _ {_ _}. { rewrite <- !vec_pos_spec, <- !vec_map_spec, <- !vec_app_spec. eapply nth_error_vec_list. 
+    cbn - [minus mult]. cbn - [minus mult] in HPREP. specialize HPREP with (m := v@[Fin.of_nat_lt Hlt]). cbn [mult] in HPREP.
+    Arguments Fin.of_nat_lt _ {_ _}. refine (HPREP _ _ _). { rewrite <- !vec_pos_spec, <- !vec_map_spec, <- !vec_app_spec. eapply nth_error_vec_list. 
     rewrite @vec_list_vec_app with (n := S k') (m := k''), vec_list_vec_map.
     rewrite nth_error_app1. 2: rewrite map_length, vec_list_length; lia.
     eapply map_nth_error.
@@ -555,12 +554,12 @@ Proof.
       rewrite <- !vec_map_spec, <- !vec_app_spec.
       rewrite !vec_list_vec_app.
       setoid_rewrite <- vec_map_spec. rewrite !vec_list_vec_map. cbn[vec_list map].
-      pose proof (@vec_list_vec_app (tape Σ) (S (k' + k'')) 4). cbn [plus] in H. rewrite H. clear H.
+      pose proof (@vec_list_vec_app (tape Σ) (S (k' + k'')) n). cbn [plus] in H. rewrite H. clear H.
       pose proof (@vec_list_vec_app (tape Σ) (S k') k''). cbn [plus] in H. rewrite H. clear H.
       rewrite !vec_list_vec_map. cbn[vec_list map]. simpl_list.
       rewrite !vec_list_cast. cbn. simpl_list. rewrite vec_list_vec_app. cbn. simpl_list. reflexivity.
     + eapply vec_list_inj. rewrite <- !vec_map_spec, <- !vec_app_spec. cbn [vec_list].
-       rewrite !vec_list_cast. 
+      rewrite !vec_list_cast.
        pose proof (@vec_list_vec_app (list bool) (S (k' + k'')) 4). cbn [plus] in H. rewrite !H. clear H.
        pose proof (@vec_list_vec_app (list bool) (S (k' + S k'')) 4). cbn [plus] in H. rewrite !H. clear H.
        cbn [vec_list app]. f_equal. rewrite !vec_list_vec_app.
@@ -579,20 +578,108 @@ Proof.
     Unshelve. exact 0.
 Qed.
 
+Lemma PREP2_spec k (Σ : finType) i s b  n : 
+  { PREP2 | forall v (t : Vector.t (tape Σ) n),
+    (i, PREP2) //
+        (i,                               ([] ::: Vector.map (fun n => repeat true n) v) +++  (@encode_bsm Σ _ t)) ->>
+        (i + length PREP2, ([] ::: Vector.const [] k                      +++  (@encode_bsm Σ _ (Vector.map (encNatTM s b) v +++ t)))) }.
+Proof.
+  unshelve eexists (BSM_cast (@PREP2' Σ s b 0 k  i n) _). abstract lia. intros v t.
+  match goal with [ |- sss_compute _ _ (_, ?st) _ ] => evar (ev : vec (list bool) (S k + 4)); enough (st = ev) as ->; subst ev end.
+    match goal with [ |- sss_compute _ _ _ (_, ?st) ] => evar (ev : vec (list bool) (S k + 4)); enough (st = ev) as ->; subst ev end.
+    rewrite <- BSM_cast_spec.
+    rewrite BSM_cast_length. eapply PREP2_spec_strong.
+    - eapply vec_list_inj.
+      rewrite <- !vec_app_spec. cbn. rewrite vec_list_cast, !vec_list_vec_app, !vec_list_const.
+      f_equal. f_equal. now rewrite NPeano.Nat.add_0_r.
+      eapply vec_list_encode_bsm. Unshelve. 3: exact [| |]. 2: exact v. 2: exact t.
+      rewrite <- !vec_map_spec, !vec_list_vec_app, !vec_list_vec_map, !vec_list_vec_app. cbn. now rewrite app_nil_r.
+    - eapply vec_list_inj.
+      rewrite <- !vec_app_spec, <- !vec_map_spec, !vec_app_cons, vec_list_cast.
+      cbn. f_equal. rewrite !vec_list_vec_app. f_equal. cbn. now simpl_list.
+      eapply vec_list_encode_bsm. f_equal.
+      eapply vec_pos_ext. intros. now rewrite vec_pos_set.
+Qed.
+
+Lemma PREP3_spec k n Σ i :
+  { PREP3 | forall v : Vector.t (list bool) k, forall t : Vector.t _ n,
+    (i, PREP3) // (i, v +++ @encode_bsm Σ _ t) ->>
+                  (i + length PREP3, v +++ (@encode_bsm Σ _ (niltape ::: t)))
+  }.
+Proof.
+  edestruct (@encode_bsm_nil Σ n) as ([str n'] & H).
+  exists (pop_many (pos_right k Fin2) n' i
+      ++ push_exactly (pos_right k Fin2) str).
+  intros v t.
+  eapply subcode_sss_compute_trans with (P := (i, pop_many (pos_right k Fin2) n' i)). auto.
+  eapply pop_many_spec.
+  eapply subcode_sss_compute_trans with (P := (n' + i, push_exactly (pos_right k Fin2) str)). 
+  { exists (pop_many (pos_right k Fin2) n' i), []. split. now rewrite app_nil_r. rewrite pop_many_length; lia. }
+  eapply push_exactly_spec. bsm sss stop.
+  f_equal. rewrite app_length, pop_many_length, push_exactly_length; lia.
+  rewrite !vec_change_idem.
+  rewrite vec_change_eq; auto.
+  rewrite <- !vec_app_spec. 
+  rewrite vec_pos_app_right.
+  eapply vec_pos_ext.  eapply pos_left_right_rect.
+  - intros p. rewrite vec_pos_app_left.
+    rewrite vec_change_neq; auto. now  rewrite vec_pos_app_left.
+  - eapply Fin4_cases.
+    + rewrite !vec_pos_app_right.
+      rewrite vec_change_neq; [ | intros ? % pos_right_inj; congruence].
+      rewrite vec_pos_app_right. now rewrite !vec_pos_spec, !encode_bsm_at0.
+    + rewrite !vec_pos_app_right.
+      rewrite vec_change_neq; [ | intros ? % pos_right_inj % pos_nxt_inj; congruence].
+      rewrite vec_pos_app_right. now rewrite !vec_pos_spec, !encode_bsm_at1.
+    + rewrite !vec_pos_app_right. 
+      rewrite vec_change_eq; auto.
+      now rewrite !vec_pos_spec, H.
+    + rewrite !vec_pos_app_right.
+      rewrite vec_change_neq; [ | intros ? % pos_right_inj % pos_nxt_inj % pos_nxt_inj; congruence].
+      rewrite vec_pos_app_right. now rewrite !vec_pos_spec, !encode_bsm_at3.
+Qed.
+
 Lemma PREP_spec k n Σ s b :
   { PREP | forall v : Vector.t nat k,
-    BSM.eval ((1 + k) + 4) (0, PREP) (0, Vector.append ([] ::: Vector.map (fun n0 : nat => repeat true n0) v) (Vector.const [] 4)) 
+    (0, PREP) // (0, Vector.append ([] ::: Vector.map (fun n0 : nat => repeat true n0) v) (Vector.const [] 4)) ->>
                                            (length PREP, Vector.append (Vector.const [] (1 + k)) ((@encode_bsm Σ _ (Vector.append (niltape ::: Vector.map (encNatTM s b) v)
                                            (Vector.const niltape n)))))
   }.
 Proof.
-Admitted.
+  destruct (PREP1_spec k Σ n) as [PREP1 H1].
+  destruct (@PREP2_spec k Σ (length PREP1) s b n) as [PREP2 H2].
+  destruct (@PREP3_spec (1 + k) (k + n) Σ (length PREP1 + length PREP2)) as [PREP3 H3].
+  exists (PREP1 ++ PREP2 ++ PREP3).
+  intros v.
+  eapply subcode_sss_compute_trans. 2: eapply H1. auto.
+  eapply subcode_sss_compute_trans. 2: eapply H2. auto.
+  eapply subcode_sss_compute_trans. 2: specialize H3 with (v := [] ## Vector.const [] k); apply H3. auto.
+  bsm sss stop. f_equal. rewrite !app_length. now rewrite plus_assoc.
+Qed.
 
-Lemma POSTP_spec m' k n (Σ : finType) s b i :
-  { POSTP | forall v : Vector.t _ k, forall t : Vector.t (tape Σ) (k + n), forall m,
-    BSM.eval ((1 + k) + (m' + 4)) (i, POSTP) (i, Vector.append ([] ## v) (Vector.append (Vector.const [] m') (encode_bsm (encNatTM s b m ## t))))
-                                            (i + length POSTP, Vector.append (repeat true m ## v) (Vector.append (Vector.const [] m') (Vector.const [] _) ))
+Lemma POSTP_spec k n (Σ : finType) s b i :
+  { POSTP | forall v : Vector.t _ k, forall t : Vector.t (tape Σ) (k + n), forall m, exists out,
+   (i, POSTP) // (i, Vector.append ([] ## v) ((encode_bsm (encNatTM s b m ## t)))) ->>
+                                            (i + length POSTP, Vector.append (repeat true m ## v) (out ))
   }.
+Proof.
+  pose (END := 0).
+  pose (THESYM := encode_sym
+  (projT1
+     (projT2
+        (FinTypeEquiv.finite_n
+           (finType_CS
+              (boundary +
+               sigList (EncodeTapes.sigTape Σ)))))
+     (inr (sigList_X (EncodeTapes.UnmarkedSymbol s))))).
+  exists (pop_many (pos_right (1 + k) Fin2) (length (strpush_common s b)) i
+      ++  pop_exactly (pos_right (1 + k) Fin2) (pos_right (1 + k) Fin0) (2 + length (strpush_common s b) + 2 * length THESYM) THESYM (i + (length (strpush_common s b)))
+      ++  PUSH (pos_right (1 + k) Fin0) true 
+      ::  POP (pos_right (1 + k) Fin0) (i + (length (strpush_common s b))) (i + (length (strpush_common s b))) :: nil).
+  intros v t m. eexists.
+  eapply subcode_sss_compute_trans. 2: eapply (pop_many_spec (pos_right (1 + k) Fin2) (length (strpush_common s b)) i). auto.
+
+  
 (* take off strpush_common *)
 (* pop unmarked symbol s, if yes increase and repeat *)
 (* if no finish *)
@@ -602,30 +689,29 @@ Theorem TM_computable_to_BSM_computable {k} (R : Vector.t nat k -> nat -> Prop) 
   TM_computable R -> BSM_computable R.
 Proof.
   intros (n & Σ & s & b & Hsb & M & HM1 & HM2) % TM_computable_iff.
-  destruct (@PREP_spec 1 k n Σ s b) as [PREP HPREP].
-  destruct (BSM_complete_simulation M (1 + k) 1 (length PREP)) as (Mbsm & Hf & Hb).
-  destruct (@POSTP_spec 1 k n Σ s b (length (PREP ++ Mbsm))) as [POSTP HPOSTP].
+  destruct (@PREP_spec k n Σ s b) as [PREP HPREP].
+  destruct (BSM_complete_simulation M (1 + k) (length PREP)) as (Mbsm & Hf & Hb).
+  destruct (@POSTP_spec k n Σ s b (length (PREP ++ Mbsm))) as [POSTP HPOSTP].
   eapply BSM_computable_iff.
   eexists. exists 0. exists (PREP ++ Mbsm ++ POSTP). split.
   - intros v m (q & t & Heval & Hhd)% HM1. eapply Hf in Heval.
     cbn in t. destruct_tapes. cbn in Hhd. subst.
     eapply BSM_sss.eval_iff in Heval. 
-    setoid_rewrite BSM_sss.eval_iff in HPREP.
-    setoid_rewrite BSM_sss.eval_iff in HPOSTP.
-    setoid_rewrite BSM_sss.eval_iff. fold plus. eexists. eexists.
+    setoid_rewrite BSM_sss.eval_iff. fold plus.
+    edestruct (HPOSTP) as [out HPOSTP'].
+    eexists. eexists.
     split.
     + eapply subcode_sss_compute_trans with (P := (0, PREP)). 1:auto.
       eapply HPREP.
       eapply subcode_sss_compute_trans with (P := (|PREP|, Mbsm)). 1:auto.
       eapply Heval.
       eapply subcode_sss_compute_trans with (P := (|PREP ++ Mbsm|, POSTP)). 1:auto.
-      rewrite <- app_length. eapply (HPOSTP (Vector.const [] k)).
+      rewrite <- app_length. eapply HPOSTP'.
       bsm sss stop. reflexivity. 
     + cbn. right. rewrite !app_length. lia.
   - intros. edestruct Hb as (? & ? & HbH). 2:eapply HM2. 2:eapply HbH.
-    setoid_rewrite BSM_sss.eval_iff in HPREP.
     eapply subcode_sss_terminates.
     2:{ eapply subcode_sss_terminates_inv. eapply bsm_sss_fun.
-        eapply H. 2: eapply HPREP. auto. }
+        eapply H. 2:{ split. eapply HPREP. cbn. lia. } auto. }
     auto.
 Qed.
